poST_model/poST_time.thy
@@ -2,6 +2,6 @@ theory poST_time
   imports Main HOL.Real
 begin
 (*days/hours/minutes/seconds/miliseconds*)
-datatype time = Time nat nat nat nat nat 
+datatype time = Time (D:nat) (H: nat) (M: nat) (S: nat) (MS: nat) 
 
 end
