poST_utils/bit_types_utils.thy
@@ -31,19 +31,230 @@ definition word_sum :: "word \<Rightarrow> word \<Rightarrow> word" where
                ((integer_of_byte var22) * 256)) in
       (byte_of_integer (divide res 256), byte_of_integer res))"
 
-
+definition byte_not :: "byte \<Rightarrow> byte" where
+  "byte_not b = byte.Byte (\<not> digit0 b) (\<not> digit1 b) (\<not> digit2 b) (\<not> digit3 b) (\<not> digit4 b) (\<not> digit5 b) (\<not> digit6 b) (\<not> digit7 b)"
 definition byte_eq :: "byte \<Rightarrow> byte \<Rightarrow> bool" where
-"byte_eq b1 b2 = (of_byte b1 = (of_byte b2 :: nat))"
+  "byte_eq b1 b2 = (of_byte b1 = (of_byte b2 :: nat))"
 definition byte_eqless :: "byte \<Rightarrow> byte \<Rightarrow> bool" where
-"byte_eqless b1 b2 = (of_byte b1 \<le> (of_byte b2 :: nat))"
+  "byte_eqless b1 b2 = (of_byte b1 \<le> (of_byte b2 :: nat))"
 definition byte_less :: "byte \<Rightarrow> byte \<Rightarrow> bool" where
-"byte_less b1 b2 = (of_byte b1 < (of_byte b2 :: nat))"
+  "byte_less b1 b2 = (of_byte b1 < (of_byte b2 :: nat))"
 definition byte_eqmore :: "byte \<Rightarrow> byte \<Rightarrow> bool" where
-"byte_eqmore b1 b2 = (of_byte b1 \<ge> (of_byte b2 :: nat))"
+  "byte_eqmore b1 b2 = (of_byte b1 \<ge> (of_byte b2 :: nat))"
 definition byte_more :: "byte \<Rightarrow> byte \<Rightarrow> bool" where
-"byte_more b1 b2 = (of_byte b1 > (of_byte b2 :: nat))"
+  "byte_more b1 b2 = (of_byte b1 > (of_byte b2 :: nat))"
 definition byte_noteq :: "byte \<Rightarrow> byte \<Rightarrow> bool" where
-"byte_noteq b1 b2 = (of_byte b1 \<noteq> (of_byte b2 :: nat))"
+  "byte_noteq b1 b2 = (of_byte b1 \<noteq> (of_byte b2 :: nat))"
+definition byte_and :: "byte \<Rightarrow> byte \<Rightarrow> byte" where
+  "byte_and b1 b2 = 
+    (Byte (digit0 b1 \<and> digit0 b2)
+          (digit1 b1 \<and> digit1 b2)
+          (digit2 b1 \<and> digit2 b2)
+          (digit3 b1 \<and> digit3 b2)
+          (digit4 b1 \<and> digit4 b2)
+          (digit5 b1 \<and> digit5 b2)
+          (digit6 b1 \<and> digit6 b2)
+          (digit7 b1 \<and> digit7 b2))"
+definition byte_or :: "byte \<Rightarrow> byte \<Rightarrow> byte" where
+  "byte_or b1 b2 = 
+    (Byte (digit0 b1 \<or> digit0 b2)
+          (digit1 b1 \<or> digit1 b2)
+          (digit2 b1 \<or> digit2 b2)
+          (digit3 b1 \<or> digit3 b2)
+          (digit4 b1 \<or> digit4 b2)
+          (digit5 b1 \<or> digit5 b2)
+          (digit6 b1 \<or> digit6 b2)
+          (digit7 b1 \<or> digit7 b2))"
+
+definition byte_xor :: "byte \<Rightarrow> byte \<Rightarrow> byte" where
+  "byte_xor b1 b2 = 
+    (Byte ((digit0 b1) \<noteq> (digit0 b2))
+          ((digit1 b1) \<noteq> (digit1 b2))
+          ((digit2 b1) \<noteq> (digit2 b2))
+          ((digit3 b1) \<noteq> (digit3 b2))
+          ((digit4 b1) \<noteq> (digit4 b2))
+          ((digit5 b1) \<noteq> (digit5 b2))
+          ((digit6 b1) \<noteq> (digit6 b2))
+          ((digit7 b1) \<noteq> (digit7 b2)))"
+
+primrec byte_arr_not :: "byte list \<Rightarrow> byte list" where
+  "byte_arr_not [] = []"
+| "byte_arr_not (b#bs) = ((byte_not b) # (byte_arr_not bs))"
+primrec byte_couple_eq :: "(byte*byte) list \<Rightarrow> bool" where
+  "byte_couple_eq [] = True" 
+| "byte_couple_eq (b#bs) = ((byte_eq (fst b) (snd b)) \<and> (byte_couple_eq bs))"
+primrec byte_couple_less :: "(byte*byte) list \<Rightarrow> bool" where
+  "byte_couple_less [] = False"
+| "byte_couple_less (b#bs) = ((byte_less (fst b) (snd b)) \<or> (byte_couple_less bs))"
+primrec byte_couple_more :: "(byte*byte) list \<Rightarrow> bool" where
+  "byte_couple_more [] = False"
+| "byte_couple_more (b#bs) = ((byte_more (fst b) (snd b)) \<or> (byte_couple_more bs))"
+definition byte_couple_eqless :: "(byte*byte) list \<Rightarrow> bool" where
+  "byte_couple_eqless ls = ((byte_couple_eq ls) \<or> (byte_couple_less ls))"
+definition byte_couple_eqmore :: "(byte*byte) list \<Rightarrow> bool" where
+  "byte_couple_eqmore ls = ((byte_couple_eq ls) \<or> (byte_couple_more ls))"
+primrec byte_couple_noteq :: "(byte*byte) list \<Rightarrow> bool" where
+  "byte_couple_noteq [] = False" 
+| "byte_couple_noteq (b#bs) = ((byte_noteq (fst b) (snd b)) \<or> (byte_couple_noteq bs))"
+primrec byte_couple_and :: "(byte*byte) list \<Rightarrow> byte list" where
+  "byte_couple_and [] = []"
+| "byte_couple_and (b#bs) = (byte_and (fst b) (snd b))#(byte_couple_and bs)"
+primrec byte_couple_or :: "(byte*byte) list \<Rightarrow> byte list" where
+  "byte_couple_or [] = []"
+| "byte_couple_or (b#bs) = (byte_or (fst b) (snd b))#(byte_couple_or bs)"
+primrec byte_couple_xor :: "(byte*byte) list \<Rightarrow> byte list" where
+  "byte_couple_xor [] = []"
+| "byte_couple_xor (b#bs) = (byte_xor (fst b) (snd b))#(byte_couple_xor bs)"
+
+definition word_not :: "word \<Rightarrow> word" where
+  "word_not w = 
+    (let (b0,b1) = w;
+         res = (byte_arr_not [b0,b1])
+      in (nth res 0, nth res 1))"
+definition word_eq :: "word \<Rightarrow> word \<Rightarrow> bool" where
+  "word_eq w1 w2 = 
+    (case (w1,w2) of
+      ((b11,b12),(b21,b22)) \<Rightarrow> (byte_couple_eq [(b11,b21),(b12,b22)]))"
+definition word_eqless :: "word \<Rightarrow> word \<Rightarrow> bool" where
+  "word_eqless w1 w2 =
+    (case (w1,w2) of
+      ((b11,b12),(b21,b22)) \<Rightarrow> (byte_couple_eqless [(b11,b21),(b12,b22)]))"
+definition word_less :: "word \<Rightarrow> word \<Rightarrow> bool" where
+  "word_less w1 w2 =
+    (case (w1,w2) of
+      ((b11,b12),(b21,b22)) \<Rightarrow> (byte_couple_less [(b11,b21),(b12,b22)]))"
+definition word_eqmore :: "word \<Rightarrow> word \<Rightarrow> bool" where
+  "word_eqmore w1 w2 =
+    (case (w1,w2) of
+      ((b11,b12),(b21,b22)) \<Rightarrow> (byte_couple_eqmore [(b11,b21),(b12,b22)]))"
+definition word_more :: "word \<Rightarrow> word \<Rightarrow> bool" where
+  "word_more w1 w2 =
+    (case (w1,w2) of
+      ((b11,b12),(b21,b22)) \<Rightarrow> (byte_couple_more [(b11,b21),(b12,b22)]))"
+definition word_noteq :: "word \<Rightarrow> word \<Rightarrow> bool" where
+  "word_noteq w1 w2 = 
+    (case (w1,w2) of
+      ((b11,b12),(b21,b22)) \<Rightarrow> (byte_couple_noteq [(b11,b21),(b12,b22)]))"
+definition word_and :: "word \<Rightarrow> word \<Rightarrow> word" where
+  "word_and w1 w2 =
+    (let (b11,b12) = w1;
+         (b21,b22) = w2;
+         res = (byte_couple_and [(b11,b21),(b12,b22)])
+     in (nth res 0, nth res 1))"
+definition word_or :: "word \<Rightarrow> word \<Rightarrow> word" where
+  "word_or w1 w2 =
+    (let (b11,b12) = w1;
+         (b21,b22) = w2;
+         res = (byte_couple_or [(b11,b21),(b12,b22)])
+     in (nth res 0, nth res 1))"
+definition word_xor :: "word \<Rightarrow> word \<Rightarrow> word" where
+  "word_xor w1 w2 =
+    (let (b11,b12) = w1;
+         (b21,b22) = w2;
+         res = (byte_couple_xor [(b11,b21),(b12,b22)])
+     in (nth res 0, nth res 1))"
+
+definition dword_not :: "dword \<Rightarrow> dword" where
+  "dword_not w= 
+    (let (b0,b1,b2,b3) = w;
+         res = (byte_arr_not [b0,b1,b2,b3])
+      in (nth res 0, nth res 1, nth res 2, nth res 3))"
+definition dword_eq :: "dword \<Rightarrow> dword \<Rightarrow> bool" where
+  "dword_eq w1 w2 = 
+    (case (w1,w2) of
+      ((b11,b12,b13,b14),(b21,b22,b23,b24)) \<Rightarrow> (byte_couple_eq [(b11,b21),(b12,b22),(b13,b23),(b14,b24)]))"
+definition dword_eqless :: "dword \<Rightarrow> dword \<Rightarrow> bool" where
+  "dword_eqless w1 w2 = 
+    (case (w1,w2) of
+      ((b11,b12,b13,b14),(b21,b22,b23,b24)) \<Rightarrow> (byte_couple_eqless [(b11,b21),(b12,b22),(b13,b23),(b14,b24)]))"
+definition dword_less :: "dword \<Rightarrow> dword \<Rightarrow> bool" where
+  "dword_less w1 w2 = 
+    (case (w1,w2) of
+      ((b11,b12,b13,b14),(b21,b22,b23,b24)) \<Rightarrow> (byte_couple_less [(b11,b21),(b12,b22),(b13,b23),(b14,b24)]))"
+definition dword_eqmore :: "dword \<Rightarrow> dword \<Rightarrow> bool" where
+  "dword_eqmore w1 w2 = 
+    (case (w1,w2) of
+      ((b11,b12,b13,b14),(b21,b22,b23,b24)) \<Rightarrow> (byte_couple_eqmore [(b11,b21),(b12,b22),(b13,b23),(b14,b24)]))"
+definition dword_more :: "dword \<Rightarrow> dword \<Rightarrow> bool" where
+  "dword_more w1 w2 = 
+    (case (w1,w2) of
+      ((b11,b12,b13,b14),(b21,b22,b23,b24)) \<Rightarrow> (byte_couple_more [(b11,b21),(b12,b22),(b13,b23),(b14,b24)]))"
+definition dword_noteq :: "dword \<Rightarrow> dword \<Rightarrow> bool" where
+  "dword_noteq w1 w2 = 
+    (case (w1,w2) of
+      ((b11,b12,b13,b14),(b21,b22,b23,b24)) \<Rightarrow> (byte_couple_noteq [(b11,b21),(b12,b22),(b13,b23),(b14,b24)]))"
+definition dword_and :: "dword \<Rightarrow> dword \<Rightarrow> dword" where
+  "dword_and w1 w2 =
+    (let (b11,b12,b13,b14) = w1;
+         (b21,b22,b23,b24) = w2;
+         res = (byte_couple_and [(b11,b21),(b12,b22),(b13,b23),(b14,b24)])
+     in (nth res 0, nth res 1, nth res 2, nth res 3))"
+definition dword_or :: "dword \<Rightarrow> dword \<Rightarrow> dword" where
+  "dword_or w1 w2 =
+    (let (b11,b12,b13,b14) = w1;
+         (b21,b22,b23,b24) = w2;
+         res = (byte_couple_or [(b11,b21),(b12,b22),(b13,b23),(b14,b24)])
+     in (nth res 0, nth res 1, nth res 2, nth res 3))"
+definition dword_xor :: "dword \<Rightarrow> dword \<Rightarrow> dword" where
+  "dword_xor w1 w2 =
+    (let (b11,b12,b13,b14) = w1;
+         (b21,b22,b23,b24) = w2;
+         res = (byte_couple_or [(b11,b21),(b12,b22),(b13,b23),(b14,b24)])
+     in (nth res 0, nth res 1, nth res 2, nth res 3))"
+
+definition lword_not :: "lword \<Rightarrow> lword" where
+"lword_not w = 
+  (let (b0,b1,b2,b3,b4,b5,b6,b7) = w;
+         res = (byte_arr_not [b0,b1,b2,b3,b4,b5,b6,b7])
+      in (nth res 0, nth res 1, nth res 2, nth res 3, nth res 4, nth res 5, nth res 6, nth res 7))"
+definition lword_eq :: "lword \<Rightarrow> lword \<Rightarrow> bool" where
+"lword_eq w1 w2 = 
+  (case (w1,w2) of
+    ((b11,b12,b13,b14,b15,b16,b17,b18),(b21,b22,b23,b24,b25,b26,b27,b28)) \<Rightarrow> 
+      (byte_couple_eq [(b11,b21),(b12,b22),(b13,b23),(b14,b24),(b15,b25),(b16,b26),(b17,b27),(b18,b28)]))"
+definition lword_eqless :: "lword \<Rightarrow> lword \<Rightarrow> bool" where
+"lword_eqless w1 w2 =
+  (case (w1,w2) of
+    ((b11,b12,b13,b14,b15,b16,b17,b18),(b21,b22,b23,b24,b25,b26,b27,b28)) \<Rightarrow> 
+      (byte_couple_eqless [(b11,b21),(b12,b22),(b13,b23),(b14,b24),(b15,b25),(b16,b26),(b17,b27),(b18,b28)]))"
+definition lword_less :: "lword \<Rightarrow> lword \<Rightarrow> bool" where
+"lword_less w1 w2 =
+  (case (w1,w2) of
+    ((b11,b12,b13,b14,b15,b16,b17,b18),(b21,b22,b23,b24,b25,b26,b27,b28)) \<Rightarrow> 
+      (byte_couple_less [(b11,b21),(b12,b22),(b13,b23),(b14,b24),(b15,b25),(b16,b26),(b17,b27),(b18,b28)]))"
+definition lword_eqmore :: "lword \<Rightarrow> lword \<Rightarrow> bool" where
+"lword_eqmore w1 w2 = 
+  (case (w1,w2) of
+    ((b11,b12,b13,b14,b15,b16,b17,b18),(b21,b22,b23,b24,b25,b26,b27,b28)) \<Rightarrow> 
+      (byte_couple_eqmore [(b11,b21),(b12,b22),(b13,b23),(b14,b24),(b15,b25),(b16,b26),(b17,b27),(b18,b28)]))"
+definition lword_more :: "lword \<Rightarrow> lword \<Rightarrow> bool" where
+"lword_more w1 w2 =
+  (case (w1,w2) of
+    ((b11,b12,b13,b14,b15,b16,b17,b18),(b21,b22,b23,b24,b25,b26,b27,b28)) \<Rightarrow> 
+      (byte_couple_more [(b11,b21),(b12,b22),(b13,b23),(b14,b24),(b15,b25),(b16,b26),(b17,b27),(b18,b28)]))"
+definition lword_noteq :: "lword \<Rightarrow> lword \<Rightarrow> bool" where
+"lword_noteq w1 w2 = 
+  (case (w1,w2) of
+    ((b11,b12,b13,b14,b15,b16,b17,b18),(b21,b22,b23,b24,b25,b26,b27,b28)) \<Rightarrow> 
+      (byte_couple_noteq [(b11,b21),(b12,b22),(b13,b23),(b14,b24),(b15,b25),(b16,b26),(b17,b27),(b18,b28)]))"
+definition lword_and :: "lword \<Rightarrow> lword \<Rightarrow> lword" where
+  "lword_and w1 w2 =
+    (let (b11,b12,b13,b14,b15,b16,b17,b18) = w1;
+         (b21,b22,b23,b24,b25,b26,b27,b28) = w2;
+         res = (byte_couple_and [(b11,b21),(b12,b22),(b13,b23),(b14,b24),(b15,b25),(b16,b26),(b17,b27),(b18,b28)])
+     in (nth res 0, nth res 1, nth res 2, nth res 3, nth res 4, nth res 5, nth res 6, nth res 7))"
+definition lword_or :: "lword \<Rightarrow> lword \<Rightarrow> lword" where
+  "lword_or w1 w2 =
+    (let (b11,b12,b13,b14,b15,b16,b17,b18) = w1;
+         (b21,b22,b23,b24,b25,b26,b27,b28) = w2;
+         res = (byte_couple_or [(b11,b21),(b12,b22),(b13,b23),(b14,b24),(b15,b25),(b16,b26),(b17,b27),(b18,b28)])
+     in (nth res 0, nth res 1, nth res 2, nth res 3, nth res 4, nth res 5, nth res 6, nth res 7))"
+definition lword_xor :: "lword \<Rightarrow> lword \<Rightarrow> lword" where
+  "lword_xor w1 w2 =
+    (let (b11,b12,b13,b14,b15,b16,b17,b18) = w1;
+         (b21,b22,b23,b24,b25,b26,b27,b28) = w2;
+         res = (byte_couple_xor [(b11,b21),(b12,b22),(b13,b23),(b14,b24),(b15,b25),(b16,b26),(b17,b27),(b18,b28)])
+     in (nth res 0, nth res 1, nth res 2, nth res 3, nth res 4, nth res 5, nth res 6, nth res 7))"
 
 end
 
