poST_lemmas/poSTVM_state_lemmas.thy
@@ -1,0 +1,160 @@
+theory poSTVM_state_lemmas
+  imports 
+    "~~/poST/poSTVM/poSTVM_state"
+    "~~/poST/poST_lemmas/ptypes_lemmas"
+begin 
+
+lemma value_mirror[simp]: "get_value (set_value st val) = val"
+  apply (induction st)
+  apply auto
+  done
+
+lemma global_vars_mirror1[simp]: "get_global_vars (set_global_vars st vars) = vars"
+  apply (induction st)
+  apply auto
+  done
+
+lemma global_vars_mirror2[simp]:
+  "(get_var_from_global_vars_by_name (set_var_in_global_vars_by_name st name val) name) = val"
+proof -
+  show ?thesis sorry
+qed
+
+lemma prog_vars_mirror1[simp]: "get_cur_prog_vars (set_cur_prog_vars st vars) = vars"
+proof - 
+  show ?thesis sorry
+qed
+  
+
+lemma prog_vars_mirror2[simp]: "(get_prog_var_by_name (set_var_in_prog_vars_by_name st name val) name) = val" 
+proof -
+  show ?thesis sorry
+qed
+
+lemma proc_vars_mirror1[simp]: "get_cur_proc_vars (set_cur_proc_vars st vars) = vars" 
+proof -
+  show ?thesis sorry
+qed
+
+lemma proc_vars_mirror2[simp]: "(get_proc_var_by_name (set_var_in_proc_vars_by_name st name val) name) = val" 
+proof -
+  show ?thesis sorry
+qed
+
+declare Let_def[simp] option.split[split]
+
+lemma set_symbvar_global_level_keep[simp]:
+  assumes "get_var_level_by_name st name = var_level.Global"
+  shows "get_var_level_by_name (set_global_var st name val) name = var_level.Global"
+proof -
+  show ?thesis sorry
+qed
+
+lemma set_symbvar_program_level_keep[simp]:
+  assumes "get_var_level_by_name st name = var_level.Program"
+  shows "get_var_level_by_name (set_cur_prog_var st name val) name = var_level.Program"
+proof -
+  show ?thesis sorry
+qed
+
+lemma set_symbvar_process_level_keep[simp]:
+  assumes "get_var_level_by_name st name = var_level.Process"
+  shows "get_var_level_by_name (set_cur_proc_var st name val) name = var_level.Process"
+proof -
+  show ?thesis sorry
+qed
+
+lemma set_symbvar_level_keep[simp]:
+  fixes level :: var_level
+  assumes "get_var_level_by_name st name = level"
+  shows "get_var_level_by_name (set_cur_symbvar st name val) name = level"
+proof (cases level)
+  case Global
+  hence "get_var_level_by_name (set_cur_symbvar st name val) name = get_var_level_by_name (set_global_var st name (stacked_var_init.Symbolic val None)) name" using assms by auto
+  then show ?thesis using set_symbvar_global_level_keep using Global assms by simp
+next
+  case Program
+  hence "get_var_level_by_name (set_cur_symbvar st name val) name = get_var_level_by_name (set_cur_prog_var st name (stacked_var_init.Symbolic val None)) name" using assms by auto
+  then show ?thesis using set_symbvar_program_level_keep using Program assms by simp
+next
+  case Process
+  hence "get_var_level_by_name (set_cur_symbvar st name val) name = get_var_level_by_name (set_cur_proc_var st name (stacked_var_init.Symbolic val None)) name" using assms by auto
+  then show ?thesis using set_symbvar_process_level_keep using Process assms by simp
+qed
+
+lemma global_var_mirror[simp]:
+  assumes "get_var_level_by_name st name = var_level.Global"
+  shows "(get_cur_var_init_by_name (set_global_var st name val) name) = val"
+proof -
+  from assms have 
+   "(get_cur_var_init_by_name (set_global_var st name val) name) = 
+    (get_var_from_global_vars_by_name (get_global_vars 
+      (set_global_var st name val)) 
+    name)" using set_symbvar_global_level_keep by auto
+  hence
+    "(get_cur_var_init_by_name (set_global_var st name val) name) =
+     (get_var_from_global_vars_by_name (get_global_vars 
+      (set_global_vars st (set_var_in_global_vars_by_name (get_global_vars st) name val))) 
+      name)" by simp
+  hence
+    "(get_cur_var_init_by_name (set_global_var st name val) name) =
+     (get_var_from_global_vars_by_name (set_var_in_global_vars_by_name (get_global_vars st) 
+      name val) name)" using global_vars_mirror1 by simp
+  thus ?thesis using global_vars_mirror2 by simp
+qed
+
+lemma program_var_mirror[simp]:
+  assumes "get_var_level_by_name st name = var_level.Program"
+  shows "(get_cur_var_init_by_name (set_cur_prog_var st name val) name) = val"
+proof -
+  from assms have
+  "(get_cur_var_init_by_name (set_cur_prog_var st name val) name) =
+    (get_prog_var_by_name (get_cur_prog_vars 
+    (set_cur_prog_var st name val)) 
+    name)" using set_symbvar_program_level_keep by auto
+  hence "(get_cur_var_init_by_name (set_cur_prog_var st name val) name) =
+          (get_prog_var_by_name (get_cur_prog_vars
+          (set_cur_prog_vars st (set_var_in_prog_vars_by_name (get_cur_prog_vars st) name val))) 
+          name)" by simp
+  hence "(get_cur_var_init_by_name (set_cur_prog_var st name val) name) =
+          (get_prog_var_by_name (set_var_in_prog_vars_by_name (get_cur_prog_vars st) name val)
+          name)" using prog_vars_mirror1 by simp
+  thus ?thesis using prog_vars_mirror2 by simp
+qed
+
+lemma process_var_mirror[simp]:
+  assumes "get_var_level_by_name st name = var_level.Process"
+  shows "(get_cur_var_init_by_name (set_cur_proc_var st name val) name) = val"
+proof -
+  from assms have
+  "(get_cur_var_init_by_name (set_cur_proc_var st name val) name) =
+    (get_proc_var_by_name (get_cur_proc_vars 
+    (set_cur_proc_var st name val)) 
+    name)" using set_symbvar_process_level_keep by auto
+  hence "(get_cur_var_init_by_name (set_cur_proc_var st name val) name) = 
+          (get_proc_var_by_name (get_cur_proc_vars 
+          (set_cur_proc_vars st (set_var_in_proc_vars_by_name (get_cur_proc_vars st) name val))) 
+           name)" by simp
+  hence "(get_cur_var_init_by_name (set_cur_proc_var st name val) name) = 
+          (get_proc_var_by_name (set_var_in_proc_vars_by_name (get_cur_proc_vars st) name val)
+          name)" using proc_vars_mirror1 by simp
+  thus ?thesis using proc_vars_mirror2 by simp
+qed
+
+lemma symbvar_mirror[simp]:
+  shows "get_cur_symbvar_by_name (set_cur_symbvar st name val) name = val"
+  
+proof (cases "(get_var_level_by_name st name)")
+  case g:Global
+  hence "get_cur_symbvar_by_name (set_cur_symbvar st name val) name = get_cur_symbvar_by_name (set_global_var st name (stacked_var_init.Symbolic val None)) name" by simp
+  from g and this show ?thesis using global_var_mirror by auto
+next
+  case p:Program
+  hence "get_cur_symbvar_by_name (set_cur_symbvar st name val) name = get_cur_symbvar_by_name (set_cur_prog_var st name (stacked_var_init.Symbolic val None)) name" by simp
+  from p and this show ?thesis using program_var_mirror by auto
+next
+  case p:Process
+  hence "get_cur_symbvar_by_name (set_cur_symbvar st name val) name = get_cur_symbvar_by_name (set_cur_proc_var st name (stacked_var_init.Symbolic val None)) name" by simp
+  from p and this show ?thesis using process_var_mirror by auto
+qed
+end
