poST_utils/poST_vars_utils.thy
@@ -4,8 +4,9 @@ begin
 
 definition basics_to_array_interval :: "ptype \<Rightarrow> ptype \<Rightarrow> array_interval" where
 "basics_to_array_interval var1 var2 = 
-  (case (ptype_to_bptint var1,ptype_to_bptint var2) of 
-    ((ptype.Int val1), (ptype.Int val2)) \<Rightarrow> array_interval.Int val1 val2)"
+  (case (var1,var2) of 
+    ((ptype.Int val1), (ptype.Int val2)) \<Rightarrow> array_interval.Int val1 val2
+  | ((ptype.Nat val1), (ptype.Nat val2)) \<Rightarrow> array_interval.Int val1 val2)"
 declare basics_to_array_interval_def [simp]
 
 end
